named_api/UnitTests/t05_non_uniform_param_types.v
@@ -2,6 +2,7 @@ From MetaCoq.Utils Require Import utils.
 From MetaCoq.Template Require Import All.
 
 From NamedAPI Require Import unit_tests.
+From NamedAPI Require Import nesting_param.
 
 
 (* nb_uparams: 0 *)
@@ -14,7 +15,7 @@ Inductive nu_list_param1 A : nu_list A -> Type :=
 | nu_cons_param1 : forall l, nu_list_param1 (A * A) l ->
                     nu_list_param1 A (nu_cons A l).
 
-MetaCoq Run (tmMsg "01/07 nu_list").
+MetaCoq Run (tmMsg "01/08 nu_list").
 Redirect "named_api/UnitTests/tests/05_01_nu_list_coq" MetaCoq Run (print_rec "nu_list" ).
 Redirect "named_api/UnitTests/tests/05_01_nu_list_gen" MetaCoq Run (generate [] nu_list).
 
@@ -28,7 +29,7 @@ Inductive mixed1_param1 A (PA : A -> Prop) B C : mixed1 A B C -> Type :=
 | mc12_param1 : forall x, mixed1_param1 A PA nat C x ->
                 mixed1_param1 A PA B C (mc12 A B C x).
 
-MetaCoq Run (tmMsg "02/07 mixed1").
+MetaCoq Run (tmMsg "02/08 mixed1").
 Redirect "named_api/UnitTests/tests/05_02_mixed1_coq" MetaCoq Run (print_rec "mixed1" ).
 Redirect "named_api/UnitTests/tests/05_02_mixed1_gen" MetaCoq Run (generate [] mixed1).
 
@@ -43,7 +44,7 @@ Inductive mixed2_param1 A B C : mixed2 A B C -> Type :=
 | mc22_param1 : forall x, mixed2_param1 nat B C x ->
                 mixed2_param1 A B C (mc22 A B C x).
 
-MetaCoq Run (tmMsg "03/07 mixed2").
+MetaCoq Run (tmMsg "03/08 mixed2").
 Redirect "named_api/UnitTests/tests/05_03_mixed2_coq" MetaCoq Run (print_rec "mixed2" ).
 Redirect "named_api/UnitTests/tests/05_03_mixed2_gen" MetaCoq Run (generate [] mixed2).
 
@@ -72,7 +73,7 @@ Inductive mixed3_param1 (A B C D : Type) : mixed3 A B C D -> Type :=
                 forall y, mixed3_param1 B A C D y ->
                 mixed3_param1 A B C D (mc35 A B C D x y).
 
-MetaCoq Run (tmMsg "04/07 mixed3").
+MetaCoq Run (tmMsg "04/08 mixed3").
 Redirect "named_api/UnitTests/tests/05_04_mixed3_coq" MetaCoq Run (print_rec "mixed3" ).
 Redirect "named_api/UnitTests/tests/05_04_mixed3_gen" MetaCoq Run (generate [] mixed3).
 
@@ -86,7 +87,7 @@ Inductive nu_vec_param1 (n : nat) : nu_vec n -> Type :=
 | vcons_pa_param1 : forall nv, nu_vec_param1 (S n) nv ->
                     nu_vec_param1 n (vcons_pa n nv).
 
-MetaCoq Run (tmMsg "05/07 nu_vec").
+MetaCoq Run (tmMsg "05/08 nu_vec").
 Redirect "named_api/UnitTests/tests/05_05_nu_vec_coq" MetaCoq Run (print_rec "nu_vec").
 Redirect "named_api/UnitTests/tests/05_05_nu_vec_gen" MetaCoq Run (generate [] nu_vec).
 
@@ -100,7 +101,7 @@ Inductive nu_ftree_param1 A : nu_ftree A -> Type :=
 | fnode_param1 : forall f, (forall n, nu_ftree_param1 (A * A) (f n)) ->
                  nu_ftree_param1 A (fnode A f).
 
-MetaCoq Run (tmMsg "06/07 nu_ftree").
+MetaCoq Run (tmMsg "06/08 nu_ftree").
 Redirect "named_api/UnitTests/tests/05_06_ftree_coq" MetaCoq Run (print_rec "nu_ftree").
 Redirect "named_api/UnitTests/tests/05_06_ftree_gen" MetaCoq Run (generate [] nu_ftree).
 
@@ -114,6 +115,25 @@ Inductive nu_ftree2_param1 A : nu_ftree2 A -> Type :=
 | fnode1_param1 : forall f, (forall n b, nu_ftree2_param1 (A * A) (f n b)) ->
                  nu_ftree2_param1 A (fnode2 A f).
 
-MetaCoq Run (tmMsg "07/07 nu_ftree2").
+MetaCoq Run (tmMsg "07/08 nu_ftree2").
 Redirect "named_api/UnitTests/tests/05_07_ftree2_coq" MetaCoq Run (print_rec "nu_ftree2").
 Redirect "named_api/UnitTests/tests/05_07_ftree2_gen" MetaCoq Run (generate [] nu_ftree2).
+
+(* nb_uparams : 3 *)
+(* strpos : [false, false, true] *)
+Inductive All2i {A B : Type} (R : nat -> A -> B -> Type) (n : nat) : list A -> list B -> Type :=
+	| All2i_nil : All2i R n [] []
+  | All2i_cons : forall (a : A) (b : B) (lA : list A) (lB : list B),
+                 R n a b -> All2i R (S n) lA lB -> All2i R n (a :: lA) (b :: lB).
+
+Inductive All2i_param1 {A B : Type} (R : nat -> A -> B -> Type) (PR : forall n a b, R n a b -> Prop)
+              (n : nat) : forall (lA : list A) (lB : list B), All2i R n lA lB -> Prop :=
+| All2i_nil_param1 : All2i_param1 R PR n [] [] (All2i_nil R n)
+| All2i_cons_param1 : forall (a : A) (b : B) (lA : list A) (lB : list B),
+                      forall (r : R n a b), PR n a b r ->
+                      forall (al : All2i R (S n) lA lB), All2i_param1 R PR (S n) lA lB al ->
+                      All2i_param1 R PR n (a :: lA) (b :: lB) (All2i_cons R n a b lA lB r al).
+
+MetaCoq Run (tmMsg "08/08 All2i").
+Redirect "named_api/UnitTests/tests/05_08_All2i_coq" MetaCoq Run (print_rec "All2i").
+Redirect "named_api/UnitTests/tests/05_08_All2i_gen" MetaCoq Run (generate Ep (@All2i)).
