named_api/API/view_args.v
@@ -2,67 +2,6 @@ From NamedAPI Require Import core.
 From NamedAPI Require Import inductive_access inductive_store.
 From NamedAPI Require Import context_access context_store.
 
-Inductive VArg :=
-| VArgIsInd     : forall (pos_indb : nat) (local :context)
-                  (local_nuprams local_indices : list term), VArg
-| VArgIsNested  : forall (xp : one_param_env) (pos_indb : nat) (local :context)
-                  (inst_uparams inst_nuparams_indices : list term), VArg
-| VArgIsFree    : forall (local : context) (hd : term), VArg.
-
-
-Unset Guard Checking.
-
-Section ViewVArgs.
-
-Context (s : state).
-Context (kname : kername).
-Context (Ep : param_env).
-
-#[local] Fixpoint view_vargs_aux (local : context) (matched : term) {struct matched} : VArg :=
-  let (hd, iargs) := decompose_app matched in
-  match hd with
-  | tProd an A B     => if #|iargs| =? 0
-                        then view_vargs_aux (local ,, vass an A) B
-                        else VArgIsFree local matched
-  | tLetIn an db A B => if #|iargs| =? 0
-                        then view_vargs_aux (local ,, vdef an db A) B
-                        else VArgIsFree local matched
-  | tInd (mkInd kname_indb pos_indb) _ =>
-    (* If it is the inductive *)
-    if eqb kname kname_indb
-    then let local_nuparams_indices := skipn (get_nb_uparams s kname) iargs in
-         let local_nuparams := firstn (get_nb_nuparams s kname) local_nuparams_indices in
-         let local_indices  := skipn  (get_nb_nuparams s kname) local_nuparams_indices in
-         VArgIsInd pos_indb local local_nuparams local_indices
-    (* 2.2 If it is nested *)
-    else if length iargs =? 0 then VArgIsFree local matched
-    else match find (fun x => eq_constant kname_indb x.(ep_kname)) Ep with
-      | Some xp =>
-        (* 2.2.1 get uparams and nuparams + indices *)
-        let inst_uparams := firstn xp.(ep_nb_uparams) iargs in
-        let inst_nuparams_indices := skipn xp.(ep_nb_uparams) iargs in
-        VArgIsNested xp pos_indb local inst_uparams inst_nuparams_indices
-      | None => VArgIsFree local matched
-      end
-  (* 3. Otherwise *)
-  | _ => VArgIsFree local matched
-  end.
-
-#[using="All"]
-Definition view_vargs (arg : term) : VArg := view_vargs_aux [] arg.
-
-
-
-
-(* A view for strictly positive argguments *)
-Inductive StrposArg :=
-| StrposArgIsUparam : forall (pos_strpos_uparams : nat) (local :context), StrposArg
-| StrposArgIsInd     : forall (pos_indb : nat) (local :context)
-                  (local_nuprams local_indices : list term), StrposArg
-| StrposArgIsNested  : forall (xp : one_param_env) (pos_indb : nat) (local :context)
-                  (inst_uparams inst_nuparams_indices : list term), StrposArg
-| StrposArgIsFree    : forall (local : context) (hd : term), StrposArg.
-
 Definition find_bool {A} (p : A -> bool) (l : list A) : nat * bool :=
 let fix aux n l :=
   match l with
@@ -71,22 +10,117 @@ let fix aux n l :=
   end in
   aux 0 l.
 
+
+
+Unset Guard Checking.
+
+Section ViewArgs.
+
+Context (s : state).
+Context (kname : kername).
+Context (Ep : param_env).
+
+(*
+
+###############################
+###    1. View Arguments    ###
+###############################
+
+*)
+
+(* 1.1 View for arguments where inductive hasn't been subsituted *)
+Inductive VArg :=
+| VArgIsInd     : forall (pos_indb : nat) (local :context)
+                  (local_nuprams local_indices : list term), VArg
+| VArgIsNested  : forall (xp : one_param_env) (pos_indb : nat) (local :context)
+                  (inst_uparams inst_nuparams_indices : list term), VArg
+| VArgIsFree    : forall (local : context) (hd : term) (iargs : list term), VArg.
+
+
+(* Set to [] is the inductive have been substituted for tInd *)
+Context (key_inds : keys).
+
+
+#[local] Fixpoint view_args_aux (local : context) (matched : term) {struct matched} : VArg :=
+  let (hd, iargs) := decompose_app matched in
+  match hd with
+  | tProd an A B     => if #|iargs| =? 0
+                        then view_args_aux (local ,, vass an A) B
+                        else VArgIsFree local hd iargs
+  | tLetIn an db A B => if #|iargs| =? 0
+                        then view_args_aux (local ,, vdef an db A) B
+                        else VArgIsFree local hd iargs
+  (* If it is the inductive *)
+  | tRel pos =>
+      match find_bool (fun k => check_pos s k pos) key_inds with
+        | (pos_strpos_uparams, true) =>
+            let local_nuparams_indices := skipn (get_nb_uparams s kname) iargs in
+            let local_nuparams := firstn (get_nb_nuparams s kname) local_nuparams_indices in
+            let local_indices  := skipn  (get_nb_nuparams s kname) local_nuparams_indices in
+            VArgIsInd pos local local_nuparams local_indices
+        | _ => VArgIsFree local hd iargs
+        end
+  (* If it is nested *)
+  | tInd (mkInd kname_indb pos_indb) _ =>
+    (* If it is the inductive *)
+    if eqb kname kname_indb
+    then let local_nuparams_indices := skipn (get_nb_uparams s kname) iargs in
+         let local_nuparams := firstn (get_nb_nuparams s kname) local_nuparams_indices in
+         let local_indices  := skipn  (get_nb_nuparams s kname) local_nuparams_indices in
+         VArgIsInd pos_indb local local_nuparams local_indices
+    (* 2.2 If it is nested *)
+    else if length iargs =? 0 then VArgIsFree local hd iargs
+    else match find (fun x => eq_constant kname_indb x.(ep_kname)) Ep with
+      | Some xp =>
+        (* 2.2.1 get uparams and nuparams + indices *)
+        let inst_uparams := firstn xp.(ep_nb_uparams) iargs in
+        let inst_nuparams_indices := skipn xp.(ep_nb_uparams) iargs in
+        VArgIsNested xp pos_indb local inst_uparams inst_nuparams_indices
+      | None => VArgIsFree local hd iargs
+      end
+  (* 3. Otherwise *)
+  | _ => VArgIsFree local hd iargs
+  end.
+
+#[using="All"]
+Definition view_args (arg : term) : VArg := view_args_aux [] arg.
+
+
+(*
+
+DOES NOT WORK !!!
+
+################################
+### 2. View UPArg Arguments ###
+################################
+
+*)
+
+(* A view for strictly positive argguments *)
+Inductive UPArg :=
+| UPArgIsUparam : forall (pos_strpos_uparams : nat) (local : context) (iargs : list term), UPArg
+| UPArgIsInd     : forall (pos_indb : nat) (local :context)
+                  (local_nuprams local_indices : list term), UPArg
+| UPArgIsNested  : forall (xp : one_param_env) (pos_indb : nat) (local :context)
+                  (inst_uparams inst_nuparams_indices : list term), UPArg
+| UPArgIsFree    : forall (local : context) (hd : term) (iargs : list term) , UPArg.
+
 Context (key_uparams : keys).
 
-Definition view_strpos_args (matched : term) : StrposArg :=
-  match view_vargs matched with
+Definition view_uparams_args (matched : term) : UPArg :=
+  match view_args matched with
   | VArgIsInd pos_indb loc local_nuparams local_indices =>
-      StrposArgIsInd pos_indb loc local_nuparams local_indices
+      UPArgIsInd pos_indb loc local_nuparams local_indices
   | VArgIsNested xp pos_indb loc local_uparams local_nuparams_indices =>
-      StrposArgIsNested xp pos_indb loc local_uparams local_nuparams_indices
-  | VArgIsFree loc m =>
-      match m with
-      | tRel n => match find_bool (fun k => check_pos s k n) key_uparams with
-                  | (pos_strpos_uparams, true) => StrposArgIsUparam pos_strpos_uparams loc
-                  | _ => StrposArgIsFree loc m
+      UPArgIsNested xp pos_indb loc local_uparams local_nuparams_indices
+  | VArgIsFree loc hd iargs =>
+      match hd with
+      | tRel pos => match find_bool (fun k => check_pos s k pos) key_uparams with
+                  | (pos_uparams, true) => UPArgIsUparam pos_uparams loc iargs
+                  | _ => UPArgIsFree loc hd iargs
                   end
-      | _ => StrposArgIsFree loc m
+      | _ => UPArgIsFree loc hd iargs
       end
   end.
 
-End ViewVArgs.
+End ViewArgs.
