named_api/Functoriality/functoriality.v
@@ -134,16 +134,16 @@ Fixpoint add_param (s : state) (strpos : list bool) (l : list term) (rc : list t
 end.
 
 Fixpoint make_func_call (s : state) (key_arg : key) (ty : term) {struct ty} : term :=
-  match view_strpos_args s kname Ep key_uparams ty with
-  | StrposArgIsUparam pos_strpos_uparams loc =>
+  match view_uparams_args s kname Ep [] key_uparams ty with
+  | UPArgIsUparam pos_uparams loc iargs =>
       let* s _ key_locals _ := closure_context_sep tLambda s (Some "locals") loc in
-      mkApp (geti_term s key_funcs pos_strpos_uparams)
+      mkApp (geti_term s key_funcs pos_uparams)
             (mkApps (get_term s key_arg) (get_terms s key_locals))
-  | StrposArgIsInd pos_indb loc local_nuparams local_indices =>
+  | UPArgIsInd pos_indb loc local_nuparams local_indices =>
       let* s _ key_locals _ := closure_context_sep tLambda s (Some "locals") loc in
       mkApp (mkApps (geti_term s key_fixs pos_indb) (local_nuparams ++ local_indices))
             (mkApps (get_term  s key_arg) (get_terms s key_locals))
-  | StrposArgIsNested xp pos_indb loc local_uparams local_nuparams_indices =>
+  | UPArgIsNested xp pos_indb loc local_uparams local_nuparams_indices =>
       let compute_nested_rc (x : term) (s s : state) : term :=
         let* s key_farg := mk_tLambda s (Some "rec_arg") (mkBindAnn nAnon Relevant) x in
         make_func_call s key_farg (lift0 1 x)
@@ -153,7 +153,7 @@ Fixpoint make_func_call (s : state) (key_arg : key) (ty : term) {struct ty} : te
       let ltm := add_param s xp.(ep_strpos_uparams) local_uparams rec_call in
           mkApp (mkApps (tConst xp.(ep_func_kname) []) (ltm ++ local_nuparams_indices))
                 (mkApps (get_term  s key_arg) (get_terms s key_locals))
-  | StrposArgIsFree loc m =>
+  | UPArgIsFree loc m iargs =>
       let* s _ key_locals _ := closure_context_sep tLambda s (Some "locals") loc in
       mkApps (get_term  s key_arg) (get_terms s key_locals)
   end.
