named_api/UnitTests/t07_nested_types.v
@@ -28,7 +28,7 @@ Inductive RoseTree_param1 A (PA : A -> Type) : RoseTree A -> Type :=
 | RTnode_param1 : forall l, list_param1 _ (fun x => RoseTree_param1 A PA x) l ->
                   RoseTree_param1 A PA (RTnode A l).
 
-MetaCoq Run (tmMsg "01/14 RoseTree").
+MetaCoq Run (tmMsg "01/15 RoseTree").
 Redirect "named_api/UnitTests/tests/07_01_RoseTree_coq" MetaCoq Run (print_rec "RoseTree").
 Redirect "named_api/UnitTests/tests/07_01_RoseTree_gen" MetaCoq Run (generate Ep RoseTree).
 
@@ -50,7 +50,7 @@ Inductive PairTree_param1 A (PA : A -> Prop) : PairTree A -> Type :=
                                         _ (fun x => PairTree_param1 A PA x) p ->
                   PairTree_param1 A PA (Pnode A p).
 
-MetaCoq Run (tmMsg "02/14 PairTree").
+MetaCoq Run (tmMsg "02/15 PairTree").
 Redirect "named_api/UnitTests/tests/07_02_PairTree_coq" MetaCoq Run (print_rec "PairTree").
 Redirect "named_api/UnitTests/tests/07_02_PairTree_gen" MetaCoq Run (generate Ep PairTree).
 
@@ -71,7 +71,7 @@ Inductive ArrowTree1_param1 A (PA : A -> Prop) : ArrowTree1 A -> Type :=
 | ATnode1_param1 : forall f, (forall b, list_param1 _ (fun x => ArrowTree1_param1 A PA x) (f b)) ->
                    ArrowTree1_param1 A PA (ATnode1 A f).
 
-MetaCoq Run (tmMsg "03/14 ArrowTree1").
+MetaCoq Run (tmMsg "03/15 ArrowTree1").
 Redirect "named_api/UnitTests/tests/07_03_ArrowTree1_coq" MetaCoq Run (print_rec "ArrowTree1").
 Redirect "named_api/UnitTests/tests/07_03_ArrowTree1_gen" MetaCoq Run (generate Ep ArrowTree1).
 
@@ -92,7 +92,7 @@ Inductive ArrowTree2_param1 A (PA : A -> Prop) : ArrowTree2 A -> Type :=
 | ATnode2_param1 : forall l, list_param1 _ (fun f => forall b, ArrowTree2_param1 A PA (f b)) l ->
                     ArrowTree2_param1 A PA (ATnode2 A l).
 
-MetaCoq Run (tmMsg "04/14 ArrowTree2").
+MetaCoq Run (tmMsg "04/15 ArrowTree2").
 Redirect "named_api/UnitTests/tests/07_04_ArrowTree2_coq" MetaCoq Run (print_rec "ArrowTree2").
 Redirect "named_api/UnitTests/tests/07_04_ArrowTree2_gen" MetaCoq Run (generate Ep ArrowTree2).
 
@@ -113,7 +113,7 @@ Inductive ArrowTree3_param1 A (PA : A -> Prop) : ArrowTree3 A -> Type :=
 | ATnode3_param1 : forall f, (forall b, list_param1 _ (fun g => forall n, ArrowTree3_param1 A PA (g n)) (f b)) ->
                     ArrowTree3_param1 A PA (ATnode3 A f).
 
-MetaCoq Run (tmMsg "05/14 ArrowTree3").
+MetaCoq Run (tmMsg "05/15 ArrowTree3").
 Redirect "named_api/UnitTests/tests/07_05_ArrowTree3_coq" MetaCoq Run (print_rec "ArrowTree3").
 Redirect "named_api/UnitTests/tests/07_05_ArrowTree3_gen" MetaCoq Run (generate Ep ArrowTree3).
 
@@ -139,7 +139,7 @@ Inductive LeftTree_param1 A (PA : A -> Prop) : LeftTree A -> Type :=
 | Lnode_param1 : forall p, prod_param1 _ (fun x => LeftTree_param1 A PA x) _ (fun _ => True) p ->
                  LeftTree_param1 A PA (Lnode A p).
 
-MetaCoq Run (tmMsg "06/14 LeftTree").
+MetaCoq Run (tmMsg "06/15 LeftTree").
 Redirect "named_api/UnitTests/tests/07_06_LeftTree_coq" MetaCoq Run (print_rec "LeftTree").
 Redirect "named_api/UnitTests/tests/07_06_LeftTree_gen" MetaCoq Run (generate Ep LeftTree).
 
@@ -162,7 +162,7 @@ Inductive RightTree_param1 A (PA : A -> Prop) : RightTree A -> Type :=
 | Rnode_param1 : forall p, prod_param1 _ (fun _ => True) _ (fun x => RightTree_param1 A PA x) p ->
                   RightTree_param1 A PA (Rnode A p).
 
-MetaCoq Run (tmMsg "07/14 RightTree").
+MetaCoq Run (tmMsg "07/15 RightTree").
 Redirect "named_api/UnitTests/tests/07_07_RightTree_coq" MetaCoq Run (print_rec "RightTree").
 Redirect "named_api/UnitTests/tests/07_07_RightTree_gen" MetaCoq Run (generate Ep RightTree).
 
@@ -188,7 +188,7 @@ Inductive NestedTree_param1 A (PA : A -> Type) : NestedTree A -> Type :=
 | Nnode_param1 : forall ll, list_param1 _ (fun l => list_param1 _ (fun x => NestedTree_param1 A PA x) l) ll ->
                  NestedTree_param1 A PA (Nnode A ll).
 
-MetaCoq Run (tmMsg "08/14 NestedTree").
+MetaCoq Run (tmMsg "08/15 NestedTree").
 Redirect "named_api/UnitTests/tests/07_08_NestedTree_coq" MetaCoq Run (print_rec "NestedTree").
 Redirect "named_api/UnitTests/tests/07_08_NestedTree_gen" MetaCoq Run (generate Ep NestedTree).
 
@@ -215,7 +215,7 @@ Inductive VecTree_param1 A (PA : A -> Type) : VecTree A -> Type :=
                   forall p, vec_param1 _ (fun x => VecTree_param1 A PA x) n p ->
                   VecTree_param1 A PA (VNnode A n p).
 
-MetaCoq Run (tmMsg "09/14 VecTree").
+MetaCoq Run (tmMsg "09/15 VecTree").
 Redirect "named_api/UnitTests/tests/07_09_VecTree_coq" MetaCoq Run (print_rec "VecTree").
 Redirect "named_api/UnitTests/tests/07_09_VecTree_gen"    MetaCoq Run (generate Ep VecTree).
 
@@ -238,7 +238,7 @@ Inductive WTree_param1 A (PA : A -> Prop) : WTree A -> Type :=
 | WTnode_param1 : forall ns, non_strpos10_param1 nat (WTree A) (fun x => WTree_param1 A PA x) 0 ns ->
                   WTree_param1 A PA (WTnode A ns).
 
-MetaCoq Run (tmMsg "10/14 WTree").
+MetaCoq Run (tmMsg "10/15 WTree").
 Redirect "named_api/UnitTests/tests/07_10_WTree_coq" MetaCoq Run (print_rec "WTree").
 Redirect "named_api/UnitTests/tests/07_10_WTree_gen" MetaCoq Run (generate Ep WTree).
 
@@ -261,7 +261,7 @@ Inductive nu_nested_param1 A (PA : A -> Prop) B C : nu_nested A B C -> Type :=
 | nu_nested_cons_pram1 : forall l, list_param1 _ (nu_nested_param1 A PA (B * B) C) l ->
                          nu_nested_param1 A PA B C (nu_nested_cons A B C l).
 
-MetaCoq Run (tmMsg "11/14 nu_nested").
+MetaCoq Run (tmMsg "11/15 nu_nested").
 Redirect "named_api/UnitTests/tests/07_11_nu_nested_coq" MetaCoq Run (print_rec "nu_nested").
 Redirect "named_api/UnitTests/tests/07_11_nu_nested_gen" MetaCoq Run (generate Ep nu_nested).
 
@@ -277,7 +277,7 @@ Inductive tricky1_param1 A (PA : A -> Prop) : tricky1 A -> Type :=
 | tricky11_param1 : forall x, prod_param1 A (fun a => PA a) nat (fun _ => True) x ->
                    tricky1_param1 A PA (tricky11 A x).
 
-(* MetaCoq Run (tmMsg "12/14 tricky1"). *)
+(* MetaCoq Run (tmMsg "12/15 tricky1"). *)
 Redirect "named_api/UnitTests/tests/07_12_tricky1_coq" MetaCoq Run (print_rec "tricky1").
 (* BUGS ISSUE UNIVERSE LEVEL *)
 (* Redirect "named_api/UnitTests/tests/07_12_tricky1_gen" MetaCoq Run (generate Ep tricky1). *)
@@ -289,7 +289,7 @@ Inductive tricky2_param1 A (PA : A -> Prop) : tricky2 A -> Type :=
 | tricky21_param1 : forall l, list_param1 A (fun a => PA a) l ->
                    tricky2_param1 A PA (tricky21 A l).
 
-(* MetaCoq Run (tmMsg "13/14 tricky2"). *)
+(* MetaCoq Run (tmMsg "13/15 tricky2"). *)
 Redirect "named_api/UnitTests/tests/07_13_tricky3_coq" MetaCoq Run (print_rec "tricky2").
 (* BUGS ISSUE UNIVERSE LEVEL *)
 (* Redirect "named_api/UnitTests/tests/07_13_tricky_gen" MetaCoq Run (generate Ep tricky2). *)
@@ -304,7 +304,18 @@ Inductive tricky3_param1 A (PA : A -> Prop) : tricky3 A -> Type :=
 | tricky32_param1 : forall x, prod_param1 (list A) (fun l => list_param1 A (fun a => PA a) l) A (fun a => PA a) x ->
             tricky3_param1 A PA (tricky32 A x).
 
-(* MetaCoq Run (tmMsg "14/14 tricky3"). *)
+(* MetaCoq Run (tmMsg "14/15 tricky3"). *)
 Redirect "named_api/UnitTests/tests/07_14_tricky3_coq" MetaCoq Run (print_rec "tricky3").
 (* BUGS ISSUE UNIVERSE LEVEL *)
 (* Redirect "named_api/UnitTests/tests/07_14_tricky_gen" MetaCoq Run (generate Ep tricky3). *)
+
+(* Nesting with a function *)
+Inductive typing {A B} (n : nat) (a : A) (b : B) : Type :=
+| typ_nil  : typing n a b
+| typ_cons : forall (lA : list A) (lB : list B),
+             All2i typing n lA lB -> typing n a b.
+
+(* MetaCoq Run (tmMsg "11/15 typing"). *)
+Redirect "named_api/UnitTests/tests/07_15_typing" MetaCoq Run (print_rec "typing").
+(* Redirect "named_api/UnitTests/tests/07_15_typing" MetaCoq Run (generate Ep (@typing)). *)
+
